theories/cancellation/CancelCore.v
@@ -2,8 +2,10 @@ Require Import CRIS.
 Require Import LMod LModTr GSim GSimFacts GSimTactics CancelTactics.
 Require Import MInline MInlineIntro MInlineElim ElimRel.
 
-Lemma cancel_core `{_crisG: !crisG Γ Σ α β τ _S _I, _concG: !concG} md sp R (e : coreE R):
-  CANCEL_GOAL md sp (trigger e) (trigger e).
+Lemma cancel_core `{_crisG: !crisG Γ Σ α β τ _S _I, _concG: !concG} md sp
+  (X: Type) (PQ: X → (Any.t → iProp Σ) * (Any.t → iProp Σ)) N mm
+  R (e : coreE R):
+  CANCEL_GOAL md sp PQ N mm (trigger e) (trigger e).
 Proof.
   r; i. destruct e.
   + iter_l. iter_r. rewrite x0 x1. s. step_r. i. step_r. step_l. exists x. step_l.
